More facts about normal order reduction paths, including the fact that the self-looping Omega term has an infinite one, and thus, by another theorem just proved, has no beta-normal-form.

examples/lambda/barendregt/chap2Script.sml
@@ -229,9 +229,10 @@ val S_def =
 val K_def = Define`K = LAM "x" (LAM "y" (VAR "x"))`;
 val I_def = Define`I = LAM "x" (VAR "x")`;
 
-val omega_def =
-    Define`omega = (LAM "x" (VAR "x" @@ VAR "x")) @@
+val Omega_def =
+    Define`Omega = (LAM "x" (VAR "x" @@ VAR "x")) @@
                      (LAM "x" (VAR "x" @@ VAR "x"))`
+val _ = Unicode.unicode_version {tmnm = "Omega", u = UnicodeChars.Omega}
 
 val SUB_LAM_RWT = store_thm(
   "SUB_LAM_RWT",
